ironfleet/src/Dafny/Distributed/Protocol/RSL/FailureProof/Phase2_PreFail/Phase2Proof_helper1.i.dfy
@@ -1,7 +1,9 @@
 include "Phase2Proof.i.dfy"
+include "GenericLemmas.i.dfy"
 
-module Rs2Phase2Proof_PostFail_Helper1 {
-import opened RslPhase2Proof_PostFail_i
+module Rs2Phase2Proof_PreFail_Helper1 {
+import opened RslPhase2Proof_PreFail_i
+import opened Rs2Phase2Proof_PreFail_Generic
 
 /* WARNING: this file a timeout of 60s to verify */
 
@@ -33,37 +35,37 @@ lemma PacketsBallotInvariant_NoReceiveStep(ts:TimestampedRslState, ts':Timestamp
     {}
 }
 
-lemma Before2a_to_Before2b(ts:TimestampedRslState, ts':TimestampedRslState, opn:OperationNumber, tios:seq<TimestampedLIoOp<NodeIdentity, RslMessage>>) 
-    requires RslAssumption(ts, opn) && RslConsistency(ts)
-    requires RslAssumption(ts', opn) && RslConsistency(ts')
-    requires PacketsBallotInvariant(ts) && PacketsBallotInvariant(ts')
-    // requires AlwaysInvariant(ts', opn)
-    requires TimestampedRslNext(ts, ts')
-    requires !TimestampedRslNextEnvironment(ts, ts')
-    requires TimestampedRslNextOneReplica(ts, ts', 1, tios);
-    requires RslPerfInvariant(ts, opn)
-    requires Before_2a_Sent_Invariant(ts, opn);
-    ensures Before_2b_Sent_Invariant(ts', opn);
-{
-    var s, s', ios := UntimestampRslState(ts), UntimestampRslState(ts'), UntagLIoOpSeq(tios);
-    var r, r' := s.replicas[1].replica, s'.replicas[1].replica;
-    var sent_packets := ExtractSentPacketsFromIos(ios);
-    var v :| 
-        (&& LValIsHighestNumberedProposal(v, r.proposer.received_1b_packets, opn)
-         && LBroadcastToEveryone(r.proposer.constants.all.config, r.proposer.constants.my_index, RslMessage_2a(r.proposer.max_ballot_i_sent_1a, opn, v), sent_packets)
-    );
-    assert |sent_packets| > 0;
-    var m := RslMessage_2a(Ballot(1, 1), opn, v);
-    assert sent_packets[0] == LPacket(r.proposer.constants.all.config.replica_ids[0], r.proposer.constants.all.config.replica_ids[1], m);
-    var pkt_witness := sent_packets[0];
-    assert LIoOpSend(pkt_witness) in ios;
-    forall pkt | pkt in ts'.t_environment.sentPackets && pkt.msg.v.RslMessage_2b?
-    ensures pkt in ts.t_environment.sentPackets
-    {}
-    assert forall p | p in sent_packets :: !p.msg.RslMessage_Reply?;
-    forall io | io in tios && io.LIoOpSend?
-    ensures !io.s.msg.v.RslMessage_Reply? {}
-}
+// lemma Before2a_to_Before2b(ts:TimestampedRslState, ts':TimestampedRslState, opn:OperationNumber, tios:seq<TimestampedLIoOp<NodeIdentity, RslMessage>>) 
+//     requires RslAssumption(ts, opn) && RslConsistency(ts)
+//     requires RslAssumption(ts', opn) && RslConsistency(ts')
+//     requires PacketsBallotInvariant(ts) && PacketsBallotInvariant(ts')
+//     // requires AlwaysInvariant(ts', opn)
+//     requires TimestampedRslNext(ts, ts')
+//     requires !TimestampedRslNextEnvironment(ts, ts')
+//     requires TimestampedRslNextOneReplica(ts, ts', 1, tios);
+//     requires RslPerfInvariant(ts, opn)
+//     requires Before_2a_Sent_Invariant(ts, opn);
+//     ensures Before_2b_Sent_Invariant(ts', opn);
+// {
+//     var s, s', ios := UntimestampRslState(ts), UntimestampRslState(ts'), UntagLIoOpSeq(tios);
+//     var r, r' := s.replicas[1].replica, s'.replicas[1].replica;
+//     var sent_packets := ExtractSentPacketsFromIos(ios);
+//     var v :| 
+//         (&& LValIsHighestNumberedProposal(v, r.proposer.received_1b_packets, opn)
+//          && LBroadcastToEveryone(r.proposer.constants.all.config, r.proposer.constants.my_index, RslMessage_2a(r.proposer.max_ballot_i_sent_1a, opn, v), sent_packets)
+//     );
+//     assert |sent_packets| > 0;
+//     var m := RslMessage_2a(Ballot(1, 1), opn, v);
+//     assert sent_packets[0] == LPacket(r.proposer.constants.all.config.replica_ids[0], r.proposer.constants.all.config.replica_ids[1], m);
+//     var pkt_witness := sent_packets[0];
+//     assert LIoOpSend(pkt_witness) in ios;
+//     forall pkt | pkt in ts'.t_environment.sentPackets && pkt.msg.v.RslMessage_2b?
+//     ensures pkt in ts.t_environment.sentPackets
+//     {}
+//     assert forall p | p in sent_packets :: !p.msg.RslMessage_Reply?;
+//     forall io | io in tios && io.LIoOpSend?
+//     ensures !io.s.msg.v.RslMessage_Reply? {}
+// }
 
 lemma Before2a_to_Before2a_NonLeaderAction(ts:TimestampedRslState, ts':TimestampedRslState, opn:OperationNumber, idx:int, tios:seq<TimestampedLIoOp<NodeIdentity, RslMessage>>) 
     requires RslAssumption(ts, opn) && RslConsistency(ts)
@@ -71,222 +73,184 @@ lemma Before2a_to_Before2a_NonLeaderAction(ts:TimestampedRslState, ts':Timestamp
     requires PacketsBallotInvariant(ts) && PacketsBallotInvariant(ts')
     requires TimestampedRslNext(ts, ts')
     requires !TimestampedRslNextEnvironment(ts, ts')
-    requires idx != 1;
+    requires idx != 0;
     requires TimestampedRslNextOneReplica(ts, ts', idx, tios);
     requires RslPerfInvariant(ts, opn)
     requires Before_2a_Sent_Invariant(ts, opn);
     ensures Before_2a_Sent_Invariant(ts', opn);
 {
-    reveal_ExtractSentPacketsFromIos();
-    reveal_UntagLIoOpSeq();
-    var ls, ls' := ts.t_replicas[idx], ts'.t_replicas[idx];
-    var nextActionIndex, nextActionIndex' := ls.v.nextActionIndex, ls'.v.nextActionIndex;
-    forall pkt | pkt in ts'.t_environment.sentPackets && pkt.msg.v.RslMessage_2a?
-    ensures pkt in ts.t_environment.sentPackets
-    {
-        if pkt !in ts.t_environment.sentPackets {
-            assert ts.t_replicas[idx].v.replica.proposer.current_state == 0;
-            if nextActionIndex == 3 {
-                assert !LProposerCanNominateUsingOperationNumber(ls.v.replica.proposer, ls.v.replica.acceptor.log_truncation_point, ls.v.replica.proposer.next_operation_number_to_propose);
-                assert forall io | io in tios :: !io.LIoOpSend?;
-                assert ts.t_environment.sentPackets == ts'.t_environment.sentPackets;
-                assert false;
-            } else {
-                forall io | io in tios && io.LIoOpSend?
-                ensures !io.s.msg.v.RslMessage_2a?
-                assert false;
-            }
-        }
-    }
-    forall pkt | pkt in ts'.t_environment.sentPackets && pkt.msg.v.RslMessage_2b?
-    ensures BalLeq(pkt.msg.v.bal_2b, Ballot(1, 0)) && pkt.msg.v.opn_2b == opn
-    {
-        if pkt !in ts.t_environment.sentPackets {
-            assert forall pkt | pkt in ts.t_environment.sentPackets && pkt.msg.v.RslMessage_2a?
-                :: BalLeq(pkt.msg.v.bal_2a, Ballot(1, 0)) && pkt.msg.v.opn_2a == opn;
-        }
-    }
-
-    forall pkt | pkt in ts'.t_environment.sentPackets 
-    ensures !IsNew2bPacket(pkt, opn) 
-    {}
-    
-    forall pkt | pkt in ts'.t_environment.sentPackets
-    ensures !IsNewReplyPacket(ts', pkt) 
-    {
-        if pkt !in ts.t_environment.sentPackets {
-            assert pkt.src == ts.constants.config.replica_ids[idx];
-            assert ReplicasDistinct(ts.constants.config.replica_ids, 1, idx);
-        }
-    }
+    assert ts'.t_replicas[0] == ts.t_replicas[0];
+    lemma_NonLeaderDoesNotSend2a(ts, ts', opn, idx, tios);
+    lemma_No2bBefore2aSent(ts, ts', opn, idx, tios);
+    lemma_NonLeaderDoesNotSendReply(ts, ts', opn, idx, tios);
 }
 
 
-lemma Before2b_to_Before2b_NonReceive(ts:TimestampedRslState, ts':TimestampedRslState, opn:OperationNumber, idx:int, tios:seq<TimestampedLIoOp<NodeIdentity, RslMessage>>) 
-    requires RslAssumption(ts, opn) && RslConsistency(ts)
-    requires RslAssumption(ts', opn) && RslConsistency(ts')
-    requires PacketsBallotInvariant(ts) && PacketsBallotInvariant(ts')
-    requires TimestampedRslNext(ts, ts')
-    requires !TimestampedRslNextEnvironment(ts, ts')
-    requires RslPerfInvariant(ts, opn)
-    requires Before_2b_Sent_Invariant(ts, opn)
-    requires TimestampedRslNextOneReplica(ts, ts', idx, tios);
-    requires ts.t_replicas[idx].v.nextActionIndex != 0
-    ensures Before_2b_Sent_Invariant(ts', opn)
-{   
-    var ls, ls' := ts.t_replicas[idx], ts'.t_replicas[idx];
-    var nextActionIndex, nextActionIndex' := ls.v.nextActionIndex, ls'.v.nextActionIndex;
+// lemma Before2b_to_Before2b_NonReceive(ts:TimestampedRslState, ts':TimestampedRslState, opn:OperationNumber, idx:int, tios:seq<TimestampedLIoOp<NodeIdentity, RslMessage>>) 
+//     requires RslAssumption(ts, opn) && RslConsistency(ts)
+//     requires RslAssumption(ts', opn) && RslConsistency(ts')
+//     requires PacketsBallotInvariant(ts) && PacketsBallotInvariant(ts')
+//     requires TimestampedRslNext(ts, ts')
+//     requires !TimestampedRslNextEnvironment(ts, ts')
+//     requires RslPerfInvariant(ts, opn)
+//     requires Before_2b_Sent_Invariant(ts, opn)
+//     requires TimestampedRslNextOneReplica(ts, ts', idx, tios);
+//     requires ts.t_replicas[idx].v.nextActionIndex != 0
+//     ensures Before_2b_Sent_Invariant(ts', opn)
+// {   
+//     var ls, ls' := ts.t_replicas[idx], ts'.t_replicas[idx];
+//     var nextActionIndex, nextActionIndex' := ls.v.nextActionIndex, ls'.v.nextActionIndex;
 
 
-    Before2b_to_Before2b_NonReceive_NoNewReply(ts, ts', opn, idx, tios);
-    forall pkt | pkt in ts'.t_environment.sentPackets
-    ensures !IsNewReplyPacket(ts', pkt) 
-    {}
+//     Before2b_to_Before2b_NonReceive_NoNewReply(ts, ts', opn, idx, tios);
+//     forall pkt | pkt in ts'.t_environment.sentPackets
+//     ensures !IsNewReplyPacket(ts', pkt) 
+//     {}
 
-    if idx != 1 {
-        forall pkt | pkt in ts'.t_environment.sentPackets && pkt.msg.v.RslMessage_2a?
-        ensures pkt in ts.t_environment.sentPackets
-        {}
-        forall pkt | pkt in ts'.t_environment.sentPackets && pkt.msg.v.RslMessage_2b?
-        ensures pkt in ts.t_environment.sentPackets
-        {
-            if pkt !in ts.t_environment.sentPackets {
-                var ios := UntagLIoOpSeq(tios);
-                var sent_packets := ExtractSentPacketsFromIos(ios);
-                assert nextActionIndex != 0;
-                assert LReplicaNoReceiveNext(ls.v.replica, nextActionIndex, ls'.v.replica, ios);
-                assert forall p | p in sent_packets :: !p.msg.RslMessage_2b?;
-                forall io | io in tios && io.LIoOpSend?
-                ensures !io.s.msg.v.RslMessage_2b? {}
-                assert false;
-            }
-        }
-        assert Before_2b_Sent_Invariant(ts', opn);
-    } else {
-        assert ts'.t_replicas[1].v.replica.learner.unexecuted_learner_state == map[];
-        assert forall opn' | opn' in ts.t_replicas[1].v.replica.learner.unexecuted_learner_state
-        ::  |ts.t_replicas[1].v.replica.learner.unexecuted_learner_state[opn].received_2b_message_senders| < LMinQuorumSize(ts.t_replicas[1].v.replica.learner.constants.all.config);
-        assert ts'.t_replicas[1].v.replica.executor == ts.t_replicas[1].v.replica.executor;
+//     if idx != 1 {
+//         forall pkt | pkt in ts'.t_environment.sentPackets && pkt.msg.v.RslMessage_2a?
+//         ensures pkt in ts.t_environment.sentPackets
+//         {}
+//         forall pkt | pkt in ts'.t_environment.sentPackets && pkt.msg.v.RslMessage_2b?
+//         ensures pkt in ts.t_environment.sentPackets
+//         {
+//             if pkt !in ts.t_environment.sentPackets {
+//                 var ios := UntagLIoOpSeq(tios);
+//                 var sent_packets := ExtractSentPacketsFromIos(ios);
+//                 assert nextActionIndex != 0;
+//                 assert LReplicaNoReceiveNext(ls.v.replica, nextActionIndex, ls'.v.replica, ios);
+//                 assert forall p | p in sent_packets :: !p.msg.RslMessage_2b?;
+//                 forall io | io in tios && io.LIoOpSend?
+//                 ensures !io.s.msg.v.RslMessage_2b? {}
+//                 assert false;
+//             }
+//         }
+//         assert Before_2b_Sent_Invariant(ts', opn);
+//     } else {
+//         assert ts'.t_replicas[1].v.replica.learner.unexecuted_learner_state == map[];
+//         assert forall opn' | opn' in ts.t_replicas[1].v.replica.learner.unexecuted_learner_state
+//         ::  |ts.t_replicas[1].v.replica.learner.unexecuted_learner_state[opn].received_2b_message_senders| < LMinQuorumSize(ts.t_replicas[1].v.replica.learner.constants.all.config);
+//         assert ts'.t_replicas[1].v.replica.executor == ts.t_replicas[1].v.replica.executor;
 
-        assert !LProposerCanNominateUsingOperationNumber(ts.t_replicas[1].v.replica.proposer, ts.t_replicas[1].v.replica.acceptor.log_truncation_point, ts.t_replicas[1].v.replica.proposer.next_operation_number_to_propose);
-        forall pkt | pkt in ts'.t_environment.sentPackets && pkt.msg.v.RslMessage_2a?
-        ensures pkt in ts.t_environment.sentPackets
-        forall pkt | pkt in ts'.t_environment.sentPackets && pkt.msg.v.RslMessage_2b?
-        ensures pkt in ts.t_environment.sentPackets
-        {
-            if pkt !in ts.t_environment.sentPackets {
-                var ios := UntagLIoOpSeq(tios);
-                var sent_packets := ExtractSentPacketsFromIos(ios);
-                assert nextActionIndex != 0;
-                assert LReplicaNoReceiveNext(ls.v.replica, nextActionIndex, ls'.v.replica, ios);
-                assert forall p | p in sent_packets :: !p.msg.RslMessage_2b?;
-                forall io | io in tios && io.LIoOpSend?
-                ensures !io.s.msg.v.RslMessage_2b? {}
-                assert false;
-            }
-        }
-        assert Before_2b_Sent_Invariant(ts', opn);
-    }
-}
-
-
-lemma Before2b_to_Before2b_NonReceive_NoNewReply(ts:TimestampedRslState, ts':TimestampedRslState, opn:OperationNumber, idx:int, tios:seq<TimestampedLIoOp<NodeIdentity, RslMessage>>) 
-    requires RslAssumption(ts, opn) && RslConsistency(ts)
-    requires RslAssumption(ts', opn) && RslConsistency(ts')
-    requires PacketsBallotInvariant(ts) && PacketsBallotInvariant(ts')
-    requires TimestampedRslNext(ts, ts')
-    requires !TimestampedRslNextEnvironment(ts, ts')
-    requires RslPerfInvariant(ts, opn)
-    requires Before_2b_Sent_Invariant(ts, opn)
-    requires TimestampedRslNextOneReplica(ts, ts', idx, tios);
-    requires ts.t_replicas[idx].v.nextActionIndex != 0
-    ensures forall pkt | pkt in ts'.t_environment.sentPackets :: !IsNewReplyPacket(ts', pkt) 
-{   
-    var ls, ls' := ts.t_replicas[idx], ts'.t_replicas[idx];
-    var nextActionIndex, nextActionIndex' := ls.v.nextActionIndex, ls'.v.nextActionIndex;
-    forall pkt | pkt in ts'.t_environment.sentPackets
-    ensures !IsNewReplyPacket(ts', pkt) 
-    {
-        if IsNewReplyPacket(ts', pkt) {
-            assert pkt !in ts.t_environment.sentPackets;
-            if nextActionIndex == 6 {
-                if idx == 1 {
-                    assert ls.v.replica.executor.next_op_to_execute == OutstandingOpUnknown();
-                    var ios := UntagLIoOpSeq(tios);
-                    var sent_packets := ExtractSentPacketsFromIos(ios);
-                    assert sent_packets == [];
-                    assert forall io | io in tios :: !io.LIoOpSend?;
-                } else {
-                    assert ReplicasDistinct(ts.constants.config.replica_ids, 1, idx);
-                    forall io | io in tios && io.LIoOpSend?
-                    ensures io.s.src != ts'.constants.config.replica_ids[1] {}
-                }
-                assert false;
-            } else {
-                var ios := UntagLIoOpSeq(tios);
-                var sent_packets := ExtractSentPacketsFromIos(ios);
-                assert nextActionIndex != 0;
-                assert forall p | p in sent_packets :: !p.msg.RslMessage_Reply?;
-                forall io | io in tios && io.LIoOpSend?
-                ensures !io.s.msg.v.RslMessage_Reply? {}
-                assert false;
-            }
-        }
-    }
-}
+//         assert !LProposerCanNominateUsingOperationNumber(ts.t_replicas[1].v.replica.proposer, ts.t_replicas[1].v.replica.acceptor.log_truncation_point, ts.t_replicas[1].v.replica.proposer.next_operation_number_to_propose);
+//         forall pkt | pkt in ts'.t_environment.sentPackets && pkt.msg.v.RslMessage_2a?
+//         ensures pkt in ts.t_environment.sentPackets
+//         forall pkt | pkt in ts'.t_environment.sentPackets && pkt.msg.v.RslMessage_2b?
+//         ensures pkt in ts.t_environment.sentPackets
+//         {
+//             if pkt !in ts.t_environment.sentPackets {
+//                 var ios := UntagLIoOpSeq(tios);
+//                 var sent_packets := ExtractSentPacketsFromIos(ios);
+//                 assert nextActionIndex != 0;
+//                 assert LReplicaNoReceiveNext(ls.v.replica, nextActionIndex, ls'.v.replica, ios);
+//                 assert forall p | p in sent_packets :: !p.msg.RslMessage_2b?;
+//                 forall io | io in tios && io.LIoOpSend?
+//                 ensures !io.s.msg.v.RslMessage_2b? {}
+//                 assert false;
+//             }
+//         }
+//         assert Before_2b_Sent_Invariant(ts', opn);
+//     }
+// }
 
 
-
+// lemma Before2b_to_Before2b_NonReceive_NoNewReply(ts:TimestampedRslState, ts':TimestampedRslState, opn:OperationNumber, idx:int, tios:seq<TimestampedLIoOp<NodeIdentity, RslMessage>>) 
+//     requires RslAssumption(ts, opn) && RslConsistency(ts)
+//     requires RslAssumption(ts', opn) && RslConsistency(ts')
+//     requires PacketsBallotInvariant(ts) && PacketsBallotInvariant(ts')
+//     requires TimestampedRslNext(ts, ts')
+//     requires !TimestampedRslNextEnvironment(ts, ts')
+//     requires RslPerfInvariant(ts, opn)
+//     requires Before_2b_Sent_Invariant(ts, opn)
+//     requires TimestampedRslNextOneReplica(ts, ts', idx, tios);
+//     requires ts.t_replicas[idx].v.nextActionIndex != 0
+//     ensures forall pkt | pkt in ts'.t_environment.sentPackets :: !IsNewReplyPacket(ts', pkt) 
+// {   
+//     var ls, ls' := ts.t_replicas[idx], ts'.t_replicas[idx];
+//     var nextActionIndex, nextActionIndex' := ls.v.nextActionIndex, ls'.v.nextActionIndex;
+//     forall pkt | pkt in ts'.t_environment.sentPackets
+//     ensures !IsNewReplyPacket(ts', pkt) 
+//     {
+//         if IsNewReplyPacket(ts', pkt) {
+//             assert pkt !in ts.t_environment.sentPackets;
+//             if nextActionIndex == 6 {
+//                 if idx == 1 {
+//                     assert ls.v.replica.executor.next_op_to_execute == OutstandingOpUnknown();
+//                     var ios := UntagLIoOpSeq(tios);
+//                     var sent_packets := ExtractSentPacketsFromIos(ios);
+//                     assert sent_packets == [];
+//                     assert forall io | io in tios :: !io.LIoOpSend?;
+//                 } else {
+//                     assert ReplicasDistinct(ts.constants.config.replica_ids, 1, idx);
+//                     forall io | io in tios && io.LIoOpSend?
+//                     ensures io.s.src != ts'.constants.config.replica_ids[1] {}
+//                 }
+//                 assert false;
+//             } else {
+//                 var ios := UntagLIoOpSeq(tios);
+//                 var sent_packets := ExtractSentPacketsFromIos(ios);
+//                 assert nextActionIndex != 0;
+//                 assert forall p | p in sent_packets :: !p.msg.RslMessage_Reply?;
+//                 forall io | io in tios && io.LIoOpSend?
+//                 ensures !io.s.msg.v.RslMessage_Reply? {}
+//                 assert false;
+//             }
+//         }
+//     }
+// }
 
 
 
-lemma Before2b_to_Before2b_Receive(ts:TimestampedRslState, ts':TimestampedRslState, opn:OperationNumber, idx:int, tios:seq<TimestampedLIoOp<NodeIdentity, RslMessage>>) 
-    requires RslAssumption(ts, opn) && RslConsistency(ts)
-    requires RslAssumption(ts', opn) && RslConsistency(ts')
-    requires PacketsBallotInvariant(ts) && PacketsBallotInvariant(ts')
-    requires TimestampedRslNext(ts, ts')
-    requires !TimestampedRslNextEnvironment(ts, ts')
-    requires RslPerfInvariant(ts, opn)
-    requires Before_2b_Sent_Invariant(ts, opn)
-    requires TimestampedRslNextOneReplica(ts, ts', idx, tios);
-    requires ts.t_replicas[idx].v.nextActionIndex == 0
-    requires !tios[0].LIoOpTimeoutReceive?
-    requires !tios[0].r.msg.v.RslMessage_2a?
-    ensures Before_2b_Sent_Invariant(ts', opn)
-{
-    reveal_ExtractSentPacketsFromIos();
-    reveal_UntagLIoOpSeq();
-    var ios := UntagLIoOpSeq(tios);
-    var sent_packets := ExtractSentPacketsFromIos(ios);
-    assert forall p | p in sent_packets :: !p.msg.RslMessage_2b?;
-    forall pkt | pkt in ts'.t_environment.sentPackets && IsNew2bPacket(pkt, opn) 
-    ensures pkt in ts.t_environment.sentPackets {
-        if pkt !in ts.t_environment.sentPackets {
-            assert UntagLPacket(pkt) in sent_packets;
-            assert false;
-        }
-    }
-    forall pkt | pkt in ts'.t_environment.sentPackets && pkt.msg.v.RslMessage_2a?
-    ensures pkt in ts.t_environment.sentPackets
-    {}
-    assert opn == ts'.t_replicas[1].v.replica.executor.ops_complete;   // Can be changed by LExecutorProcessAppStateSupply packet
-    assert BalLt(ts'.t_replicas[1].v.replica.learner.max_ballot_seen, Ballot(1, 1)); 
-    forall pkt | pkt in ts'.t_environment.sentPackets && IsNewReplyPacket(ts', pkt) 
-    ensures pkt in ts.t_environment.sentPackets
-    {}
 
-    forall pkt | pkt in ts'.undeliveredPackets && IsNew2aPacket(pkt, opn)
-    ensures TimeLe(pkt.msg.ts, TimeBound2aDeliveryPost())
-    {
-        if pkt !in ts.undeliveredPackets {
-            forall io | io in tios && io.LIoOpSend?
-            ensures !io.s.msg.v.RslMessage_2a?
-            assert false;
-        }
-    }
 
-    assert Before_2b_Sent_Invariant(ts', opn);
-}
+
+// lemma Before2b_to_Before2b_Receive(ts:TimestampedRslState, ts':TimestampedRslState, opn:OperationNumber, idx:int, tios:seq<TimestampedLIoOp<NodeIdentity, RslMessage>>) 
+//     requires RslAssumption(ts, opn) && RslConsistency(ts)
+//     requires RslAssumption(ts', opn) && RslConsistency(ts')
+//     requires PacketsBallotInvariant(ts) && PacketsBallotInvariant(ts')
+//     requires TimestampedRslNext(ts, ts')
+//     requires !TimestampedRslNextEnvironment(ts, ts')
+//     requires RslPerfInvariant(ts, opn)
+//     requires Before_2b_Sent_Invariant(ts, opn)
+//     requires TimestampedRslNextOneReplica(ts, ts', idx, tios);
+//     requires ts.t_replicas[idx].v.nextActionIndex == 0
+//     requires !tios[0].LIoOpTimeoutReceive?
+//     requires !tios[0].r.msg.v.RslMessage_2a?
+//     ensures Before_2b_Sent_Invariant(ts', opn)
+// {
+//     reveal_ExtractSentPacketsFromIos();
+//     reveal_UntagLIoOpSeq();
+//     var ios := UntagLIoOpSeq(tios);
+//     var sent_packets := ExtractSentPacketsFromIos(ios);
+//     assert forall p | p in sent_packets :: !p.msg.RslMessage_2b?;
+//     forall pkt | pkt in ts'.t_environment.sentPackets && IsNew2bPacket(pkt, opn) 
+//     ensures pkt in ts.t_environment.sentPackets {
+//         if pkt !in ts.t_environment.sentPackets {
+//             assert UntagLPacket(pkt) in sent_packets;
+//             assert false;
+//         }
+//     }
+//     forall pkt | pkt in ts'.t_environment.sentPackets && pkt.msg.v.RslMessage_2a?
+//     ensures pkt in ts.t_environment.sentPackets
+//     {}
+//     assert opn == ts'.t_replicas[1].v.replica.executor.ops_complete;   // Can be changed by LExecutorProcessAppStateSupply packet
+//     assert BalLt(ts'.t_replicas[1].v.replica.learner.max_ballot_seen, Ballot(1, 1)); 
+//     forall pkt | pkt in ts'.t_environment.sentPackets && IsNewReplyPacket(ts', pkt) 
+//     ensures pkt in ts.t_environment.sentPackets
+//     {}
+
+//     forall pkt | pkt in ts'.undeliveredPackets && IsNew2aPacket(pkt, opn)
+//     ensures TimeLe(pkt.msg.ts, TimeBound2aDeliveryPost())
+//     {
+//         if pkt !in ts.undeliveredPackets {
+//             forall io | io in tios && io.LIoOpSend?
+//             ensures !io.s.msg.v.RslMessage_2a?
+//             assert false;
+//         }
+//     }
+
+//     assert Before_2b_Sent_Invariant(ts', opn);
+// }
 
 
 }
