ironfleet/src/Dafny/Distributed/Protocol/RSL/FailureProof/Phase2_PreFail/Phase2Proof_toplevel.i.dfy
@@ -1,13 +1,13 @@
 include "Phase2Proof.i.dfy"
 include "Phase2Proof_helper0.i.dfy"
 include "Phase2Proof_helper1.i.dfy"
-include "Phase2Proof_helper2.i.dfy"
+// include "Phase2Proof_helper2.i.dfy"
 
-module Rs2Phase2Proof_PostFail_Top {
-import opened RslPhase2Proof_PostFail_i
-import opened Rs2Phase2Proof_PostFail_Helper0
-import opened Rs2Phase2Proof_PostFail_Helper1
-import opened Rs2Phase2Proof_PostFail_Helper2
+module Rs2Phase2Proof_PreFail_Top {
+import opened RslPhase2Proof_PreFail_i
+import opened Rs2Phase2Proof_PreFail_Helper0
+import opened Rs2Phase2Proof_PreFail_Helper1
+// import opened Rs2Phase2Proof_PostFail_Helper2
 
 
 /**** MAIN INVARIANT THEOREM ****/
@@ -21,17 +21,20 @@ lemma PerfInvariantMaintained(s:TimestampedRslState, s':TimestampedRslState, req
     PacketsBallotInvariant_Maintained(s, s', opn);
     AlwaysInvariant_Maintained(s, s', opn);
     
-    if  && (!exists pkt :: pkt in s.t_environment.sentPackets && IsNew2aPacket(pkt, opn))
-        && (!exists pkt :: pkt in s.t_environment.sentPackets && IsNew2bPacket(pkt, opn)) 
+    if  && (!exists pkt :: pkt in s.t_environment.sentPackets && IsPreFail2aPacket(pkt, opn))
+        && (!exists pkt :: pkt in s.t_environment.sentPackets && IsPreFail2bPacket(pkt, opn)) 
     {
         Before2a_to_MaybeBefore2b(s, s', opn);
-    } else if (exists pkt :: pkt in s.t_environment.sentPackets && IsNew2aPacket(pkt, opn))
-        && (!exists pkt :: pkt in s.t_environment.sentPackets && IsNew2bPacket(pkt, opn))  
+    } else if (exists pkt :: pkt in s.t_environment.sentPackets && IsPreFail2aPacket(pkt, opn))
+        && (!exists pkt :: pkt in s.t_environment.sentPackets && IsPreFail2bPacket(pkt, opn))  
     {
-        Before2b_to_MaybeAfter2b(s, s', opn);
+        // TODO
+        assume false;
+        // Before2b_to_MaybeAfter2b(s, s', opn);
     } else {
-        assert After_2b_Sent_Invariant(s, opn);
-        After2b_to_After2b(s, s', opn);
+        assume false;
+        // assert After_2b_Sent_Invariant(s, opn);
+        // After2b_to_After2b(s, s', opn);
     }
     assert RslPerfInvariant(s', opn);
 }
@@ -82,74 +85,77 @@ lemma Before2a_to_MaybeBefore2b(ts:TimestampedRslState, ts':TimestampedRslState,
     }
     var idx, tios:seq<TimestampedLIoOp<NodeIdentity, RslMessage>> :| TimestampedRslNextOneReplica(ts, ts', idx, tios);
     var nextActionIndex := ts.t_replicas[idx].v.nextActionIndex;
-    if idx != 1 {
+    if idx != 0 {
         Before2a_to_Before2a_NonLeaderAction(ts, ts', opn, idx, tios);
         return;
     }
-    Before2a_to_Before2b(ts, ts', opn, tios);
+
+    // TODO
+    assume false;
+    // Before2a_to_Before2b(ts, ts', opn, tios);
 }
 
 
-/* Proof that a Before_2b_Sent state transitions to a Before_2b_Sent state or 
-* After_2b_Sent state */
-lemma Before2b_to_MaybeAfter2b(ts:TimestampedRslState, ts':TimestampedRslState, opn:OperationNumber) 
-    requires RslAssumption(ts, opn) && RslConsistency(ts)
-    requires RslAssumption(ts', opn) && RslConsistency(ts')
-    requires PacketsBallotInvariant(ts) && PacketsBallotInvariant(ts')
-    requires AlwaysInvariant(ts', opn)
-    requires TimestampedRslNext(ts, ts')
-    requires RslPerfInvariant(ts, opn)
-    requires Before_2b_Sent_Invariant(ts, opn)
-    ensures Before_2b_Sent_Invariant(ts', opn) || After_2b_Sent_Invariant(ts', opn)
-{
-    if TimestampedRslNextEnvironment(ts, ts') {
-        assert Before_2b_Sent_Invariant(ts', opn);
-        return;
-    }
-    var idx, tios:seq<TimestampedLIoOp<NodeIdentity, RslMessage>> :| TimestampedRslNextOneReplica(ts, ts', idx, tios);
-    var nextActionIndex := ts.t_replicas[idx].v.nextActionIndex;
-    if nextActionIndex != 0 {
-        Before2b_to_Before2b_NonReceive(ts, ts', opn, idx, tios);
-        return;
-    }
-    // From this point on, nextActionIndex == 0
-    var s, s', ios := UntimestampRslState(ts), UntimestampRslState(ts'), UntagLIoOpSeq(tios);
-    var r, r' := s.replicas[idx].replica, s'.replicas[idx].replica;
-    if ios[0].LIoOpTimeoutReceive? {
-        assert ts'.t_environment.sentPackets == ts.t_environment.sentPackets;
-        assert Before_2b_Sent_Invariant(ts', opn);
-        return;
-    }
-    var sent_packets := ExtractSentPacketsFromIos(ios);
-    if !ios[0].r.msg.RslMessage_2a? {
-        Before2b_to_Before2b_Receive(ts, ts', opn, idx, tios);
-        return;
-    }
-    // From this point on, replica idx is processing a 2a packet
-    Before2b_to_MaybeAfter2b_Process2a(ts, ts', opn, idx, tios);
-}
+// /* Proof that a Before_2b_Sent state transitions to a Before_2b_Sent state or 
+// * After_2b_Sent state */
+// lemma Before2b_to_MaybeAfter2b(ts:TimestampedRslState, ts':TimestampedRslState, opn:OperationNumber) 
+//     requires RslAssumption(ts, opn) && RslConsistency(ts)
+//     requires RslAssumption(ts', opn) && RslConsistency(ts')
+//     requires PacketsBallotInvariant(ts) && PacketsBallotInvariant(ts')
+//     requires AlwaysInvariant(ts', opn)
+//     requires TimestampedRslNext(ts, ts')
+//     requires RslPerfInvariant(ts, opn)
+//     requires Before_2b_Sent_Invariant(ts, opn)
+//     ensures Before_2b_Sent_Invariant(ts', opn) || After_2b_Sent_Invariant(ts', opn)
+// {
+//     if TimestampedRslNextEnvironment(ts, ts') {
+//         assert Before_2b_Sent_Invariant(ts', opn);
+//         return;
+//     }
+//     var idx, tios:seq<TimestampedLIoOp<NodeIdentity, RslMessage>> :| TimestampedRslNextOneReplica(ts, ts', idx, tios);
+//     var nextActionIndex := ts.t_replicas[idx].v.nextActionIndex;
+//     if nextActionIndex != 0 {
+//         Before2b_to_Before2b_NonReceive(ts, ts', opn, idx, tios);
+//         return;
+//     }
+//     // From this point on, nextActionIndex == 0
+//     var s, s', ios := UntimestampRslState(ts), UntimestampRslState(ts'), UntagLIoOpSeq(tios);
+//     var r, r' := s.replicas[idx].replica, s'.replicas[idx].replica;
+//     if ios[0].LIoOpTimeoutReceive? {
+//         assert ts'.t_environment.sentPackets == ts.t_environment.sentPackets;
+//         assert Before_2b_Sent_Invariant(ts', opn);
+//         return;
+//     }
+//     var sent_packets := ExtractSentPacketsFromIos(ios);
+//     if !ios[0].r.msg.RslMessage_2a? {
+//         Before2b_to_Before2b_Receive(ts, ts', opn, idx, tios);
+//         return;
+//     }
+//     // From this point on, replica idx is processing a 2a packet
+//     Before2b_to_MaybeAfter2b_Process2a(ts, ts', opn, idx, tios);
+// }
 
 
-/* Proof that a After_2b_Sent state transitions to a After_2b_Sent state */
-lemma After2b_to_After2b(ts:TimestampedRslState, ts':TimestampedRslState, opn:OperationNumber) 
-    requires RslAssumption(ts, opn) && RslConsistency(ts)
-    requires RslAssumption(ts', opn) && RslConsistency(ts')
-    requires PacketsBallotInvariant(ts) && PacketsBallotInvariant(ts')
-    requires AlwaysInvariant(ts', opn)
-    requires TimestampedRslNext(ts, ts')
-    requires RslPerfInvariant(ts, opn)
-    requires After_2b_Sent_Invariant(ts, opn)
-    ensures After_2b_Sent_Invariant(ts', opn)
-{
-    if TimestampedRslNextEnvironment(ts, ts') {
-        assert After_2b_Sent_Invariant(ts', opn);
-        return;
-    }
-    var idx, tios:seq<TimestampedLIoOp<NodeIdentity, RslMessage>> :| TimestampedRslNextOneReplica(ts, ts', idx, tios);
-    if idx == 1 {
-        After2b_to_After2b_LeaderAction(ts, ts', opn, idx, tios);
-    } else {
-        After2b_to_After2b_NonLeaderAction(ts, ts', opn, idx, tios);
-    }
-}
+// /* Proof that a After_2b_Sent state transitions to a After_2b_Sent state */
+// lemma After2b_to_After2b(ts:TimestampedRslState, ts':TimestampedRslState, opn:OperationNumber) 
+//     requires RslAssumption(ts, opn) && RslConsistency(ts)
+//     requires RslAssumption(ts', opn) && RslConsistency(ts')
+//     requires PacketsBallotInvariant(ts) && PacketsBallotInvariant(ts')
+//     requires AlwaysInvariant(ts', opn)
+//     requires TimestampedRslNext(ts, ts')
+//     requires RslPerfInvariant(ts, opn)
+//     requires After_2b_Sent_Invariant(ts, opn)
+//     ensures After_2b_Sent_Invariant(ts', opn)
+// {
+//     if TimestampedRslNextEnvironment(ts, ts') {
+//         assert After_2b_Sent_Invariant(ts', opn);
+//         return;
+//     }
+//     var idx, tios:seq<TimestampedLIoOp<NodeIdentity, RslMessage>> :| TimestampedRslNextOneReplica(ts, ts', idx, tios);
+//     if idx == 1 {
+//         After2b_to_After2b_LeaderAction(ts, ts', opn, idx, tios);
+//     } else {
+//         After2b_to_After2b_NonLeaderAction(ts, ts', opn, idx, tios);
+//     }
+// }
 }
