ironfleet/src/Dafny/Distributed/Protocol/RSL/FailureProof/Phase2_PreFail/verify.sh
@@ -1,0 +1,25 @@
+#!/bin/bash -li
+
+
+echo "Verifying GenericLemmas.i.dfy"
+dafny GenericLemmas.i.dfy | grep -iv "Warning"
+
+# echo ""
+# echo "Verifying (long) Phase2Proof_helper0.i.dfy"
+# dafnylong Phase2Proof_helper0.i.dfy | grep -iv "Warning"
+
+echo ""
+echo "Verifying (long) Phase2Proof_helper1.i.dfy"
+dafnylong Phase2Proof_helper1.i.dfy | grep -iv "Warning"
+
+# echo ""
+# echo "Verifying (long) Phase2Proof_helper2.i.dfy"
+# dafnylong Phase2Proof_helper2.i.dfy | grep -iv "Warning"
+
+echo ""
+echo "Verifying Phase2Proof.i.dfy"
+dafny Phase2Proof.i.dfy | grep -iv "Warning"
+
+echo ""
+echo "Verifying Phase2Proof_toplevel.i.dfy"
+dafny Phase2Proof_toplevel.i.dfy | grep -iv "Warning"
